derived_then.thy
@@ -5,8 +5,12 @@ begin
 
 \<comment> \<open>Annoying: cannot call this "then" as it is a keyword\<close>
 
+definition b_then2 :: "'\<alpha> bidef \<Rightarrow> '\<beta> bidef \<Rightarrow> ('\<alpha> \<times> '\<beta>) bidef" where
+  "b_then2 ab bb = dep_then ab (\<lambda>a. transform (\<lambda> b. (a, b)) (\<lambda> (a', b). b) bb) (\<lambda> (a', b). a')"
+
+
 definition b_then :: "'\<alpha> bidef \<Rightarrow> '\<beta> bidef \<Rightarrow> ('\<alpha> \<times> '\<beta>) bidef" where
-  "b_then ab bb = dep_then ab (\<lambda>a. transform (\<lambda> b. (a, b)) (\<lambda> (a', b). b) bb) (\<lambda> (a', b). a')"
+  "b_then ab bb = dep_then ab (\<lambda>a. transform (Pair a) snd bb) fst"
 
 
 
@@ -43,6 +47,51 @@ lemma b_then_p_has_result[fp_NER]:
 
 
 \<comment> \<open>well formed\<close>
+
+definition pa_does_not_eat_into_pb_nondep :: "'\<alpha> bidef \<Rightarrow> '\<beta> bidef \<Rightarrow> bool" where
+  "pa_does_not_eat_into_pb_nondep ba bb \<longleftrightarrow> (
+    \<forall> t1 pr1 t2 pr2. p_has_result (print ba) t1 pr1 \<and> p_has_result (print bb) t2 pr2
+        \<longrightarrow> has_result (parse ba) (pr1@pr2) t1 pr2
+)"
+
+
+lemma b_then_wf_derived:
+  assumes "bidef_well_formed b1"
+  assumes "bidef_well_formed b2"
+  assumes "pa_does_not_eat_into_pb_nondep b1 b2"
+  shows "bidef_well_formed (b_then b1 b2)"
+  unfolding b_then_def
+  apply (rule dep_then_well_formed)
+  subgoal by (rule assms(1))
+  subgoal
+    unfolding well_formed_dep_then_pair_def
+    apply (rule conjI3)
+    subgoal
+      unfolding b2_wf_for_all_res_of_b1_def
+                bidef_well_formed_def
+                parser_can_parse_print_result_def
+                printer_can_print_parse_result_def
+      apply (clarsimp)
+      using assms(2)[unfolded bidef_well_formed_def parser_can_parse_print_result_def printer_can_print_parse_result_def]
+            assms(3)[unfolded pa_does_not_eat_into_pb_nondep_def]
+      apply (auto simp add: NER_simps fp_NER)
+      subgoal for i ra la b x a
+        (* Nitpick finds a counterexample here. *)
+        sorry
+      subgoal by (metis snd_conv transform_p_has_result(1))
+      done
+    subgoal
+      unfolding reversed_b2_result_is_b1_result_def
+      by (simp add: NER_simps)
+    subgoal
+      unfolding pa_does_not_eat_into_pb_def
+      using assms(3)[unfolded pa_does_not_eat_into_pb_nondep_def]
+            assms(2)[unfolded bidef_well_formed_def]
+      by (auto simp add: NER_simps fp_NER)
+    done
+  oops
+
+
 \<comment> \<open>For all the parse results that the two can have, ensure that they can be re-parsed from the text if appended.\<close>
 definition well_formed_b_then_pair :: "'\<alpha> bidef \<Rightarrow> '\<beta> bidef \<Rightarrow> bool" where
   "well_formed_b_then_pair b1 b2 \<longleftrightarrow>
@@ -55,15 +104,18 @@ lemma b_then_well_formed:
   assumes "bidef_well_formed b1"
   assumes "bidef_well_formed b2"
   assumes "well_formed_b_then_pair b1 b2"
+  assumes "pa_does_not_eat_into_pb_nondep b1 b2"
   shows   "bidef_well_formed (b_then b1 b2)"
   apply wf_init
   subgoal
-    using assms(3)
+    using assms(3, 3)
     unfolding parser_can_parse_print_result_def
               well_formed_b_then_pair_def
+              pa_does_not_eat_into_pb_nondep_def
     apply (unfold b_then_has_result(3))
     apply (unfold b_then_p_has_result(3))
-    by fast
+    apply auto
+    by (meson assms(2) assms(4) bidef_well_formed_def pa_does_not_eat_into_pb_nondep_def parser_can_parse_print_result_def)
   subgoal
     using assms(1,2)
     unfolding printer_can_print_parse_result_def
