all_definitions.thy
@@ -17,7 +17,7 @@ begin
 text \<open>
 This is the second collation phase of the dependency graph.
 Importing this files give you all the basic and the derived definitions.
-The intention is for this file to be the entrypoint to the library.
+The intention is for this file to be the entry point to the library.
 So the examples will also import this file to start.
 The dependency graph should contain as much parallelism as attainable using the
  "multiple diamond" structure as explained in the basic definitions file.
